strated ttt

.lake/build/ir/Games/gameLib/Zermelo.c
@@ -1,0 +1,108 @@
+// Lean compiler output
+// Module: Games.gameLib.Zermelo
+// Imports: Init Games.gameLib.Basic Mathlib.Tactic
+#include <lean/lean.h>
+#if defined(__clang__)
+#pragma clang diagnostic ignored "-Wunused-parameter"
+#pragma clang diagnostic ignored "-Wunused-label"
+#elif defined(__GNUC__) && !defined(__CLANG__)
+#pragma GCC diagnostic ignored "-Wunused-parameter"
+#pragma GCC diagnostic ignored "-Wunused-label"
+#pragma GCC diagnostic ignored "-Wunused-but-set-variable"
+#endif
+#ifdef __cplusplus
+extern "C" {
+#endif
+LEAN_EXPORT lean_object* l_Game__World_world__after__fst___elambda__2___rarg(lean_object*, lean_object*, lean_object*);
+LEAN_EXPORT lean_object* l_Game__World_world__after__fst___rarg(lean_object*, lean_object*);
+LEAN_EXPORT lean_object* l_Game__World_world__after__fst___elambda__1___rarg(lean_object*, lean_object*, lean_object*);
+LEAN_EXPORT lean_object* l_Game__World_world__after__fst___elambda__2(lean_object*, lean_object*);
+LEAN_EXPORT lean_object* l_Game__World_world__after__fst(lean_object*, lean_object*);
+LEAN_EXPORT lean_object* l_Game__World_world__after__fst___elambda__1(lean_object*, lean_object*);
+LEAN_EXPORT lean_object* l_Game__World_world__after__fst___elambda__1___rarg(lean_object* x_1, lean_object* x_2, lean_object* x_3) {
+_start:
+{
+lean_object* x_4; lean_object* x_5; 
+x_4 = lean_ctor_get(x_1, 2);
+lean_inc(x_4);
+lean_dec(x_1);
+x_5 = lean_apply_2(x_4, x_2, x_3);
+return x_5;
+}
+}
+LEAN_EXPORT lean_object* l_Game__World_world__after__fst___elambda__1(lean_object* x_1, lean_object* x_2) {
+_start:
+{
+lean_object* x_3; 
+x_3 = lean_alloc_closure((void*)(l_Game__World_world__after__fst___elambda__1___rarg), 3, 0);
+return x_3;
+}
+}
+LEAN_EXPORT lean_object* l_Game__World_world__after__fst___elambda__2___rarg(lean_object* x_1, lean_object* x_2, lean_object* x_3) {
+_start:
+{
+lean_object* x_4; lean_object* x_5; 
+x_4 = lean_ctor_get(x_1, 1);
+lean_inc(x_4);
+lean_dec(x_1);
+x_5 = lean_apply_2(x_4, x_2, x_3);
+return x_5;
+}
+}
+LEAN_EXPORT lean_object* l_Game__World_world__after__fst___elambda__2(lean_object* x_1, lean_object* x_2) {
+_start:
+{
+lean_object* x_3; 
+x_3 = lean_alloc_closure((void*)(l_Game__World_world__after__fst___elambda__2___rarg), 3, 0);
+return x_3;
+}
+}
+LEAN_EXPORT lean_object* l_Game__World_world__after__fst___rarg(lean_object* x_1, lean_object* x_2) {
+_start:
+{
+lean_object* x_3; lean_object* x_4; lean_object* x_5; lean_object* x_6; lean_object* x_7; 
+lean_inc(x_1);
+x_3 = lean_alloc_closure((void*)(l_Game__World_world__after__fst___elambda__2___rarg), 3, 1);
+lean_closure_set(x_3, 0, x_1);
+x_4 = lean_box(0);
+lean_inc(x_1);
+x_5 = l_Game__World_world__after__fst___elambda__2___rarg(x_1, x_4, x_2);
+x_6 = lean_alloc_closure((void*)(l_Game__World_world__after__fst___elambda__1___rarg), 3, 1);
+lean_closure_set(x_6, 0, x_1);
+x_7 = lean_alloc_ctor(0, 3, 0);
+lean_ctor_set(x_7, 0, x_5);
+lean_ctor_set(x_7, 1, x_3);
+lean_ctor_set(x_7, 2, x_6);
+return x_7;
+}
+}
+LEAN_EXPORT lean_object* l_Game__World_world__after__fst(lean_object* x_1, lean_object* x_2) {
+_start:
+{
+lean_object* x_3; 
+x_3 = lean_alloc_closure((void*)(l_Game__World_world__after__fst___rarg), 2, 0);
+return x_3;
+}
+}
+lean_object* initialize_Init(uint8_t builtin, lean_object*);
+lean_object* initialize_Games_gameLib_Basic(uint8_t builtin, lean_object*);
+lean_object* initialize_Mathlib_Tactic(uint8_t builtin, lean_object*);
+static bool _G_initialized = false;
+LEAN_EXPORT lean_object* initialize_Games_gameLib_Zermelo(uint8_t builtin, lean_object* w) {
+lean_object * res;
+if (_G_initialized) return lean_io_result_mk_ok(lean_box(0));
+_G_initialized = true;
+res = initialize_Init(builtin, lean_io_mk_world());
+if (lean_io_result_is_error(res)) return res;
+lean_dec_ref(res);
+res = initialize_Games_gameLib_Basic(builtin, lean_io_mk_world());
+if (lean_io_result_is_error(res)) return res;
+lean_dec_ref(res);
+res = initialize_Mathlib_Tactic(builtin, lean_io_mk_world());
+if (lean_io_result_is_error(res)) return res;
+lean_dec_ref(res);
+return lean_io_result_mk_ok(lean_box(0));
+}
+#ifdef __cplusplus
+}
+#endif
