.lake/build/ir/Games/games/PickUpBricks.c
@@ -1,0 +1,392 @@
+// Lean compiler output
+// Module: Games.games.PickUpBricks
+// Imports: Init Games.exLib.Nat Games.gameLib.Basic Mathlib.Tactic
+#include <lean/lean.h>
+#if defined(__clang__)
+#pragma clang diagnostic ignored "-Wunused-parameter"
+#pragma clang diagnostic ignored "-Wunused-label"
+#elif defined(__GNUC__) && !defined(__CLANG__)
+#pragma GCC diagnostic ignored "-Wunused-parameter"
+#pragma GCC diagnostic ignored "-Wunused-label"
+#pragma GCC diagnostic ignored "-Wunused-but-set-variable"
+#endif
+#ifdef __cplusplus
+extern "C" {
+#endif
+static lean_object* l_PickUpBricks__pubWin__vs__toy___closed__4;
+LEAN_EXPORT lean_object* l_toy__strat___boxed(lean_object*, lean_object*);
+LEAN_EXPORT lean_object* l_bricks__end__turn__from__ini__hist__act(lean_object*, lean_object*, lean_object*);
+LEAN_EXPORT lean_object* l___private_Games_games_PickUpBricks_0__PickUpBricks_match__1_splitter(lean_object*);
+LEAN_EXPORT lean_object* l___private_Games_games_PickUpBricks_0__History__on__turn_match__1_splitter___rarg(lean_object*, lean_object*, lean_object*);
+lean_object* l_List_foldl___at_Composition_sizeUpTo___spec__2(lean_object*, lean_object*);
+static lean_object* l_PickUpBricks__pubWin__vs__toy___closed__2;
+LEAN_EXPORT lean_object* l_PickUpBricks___elambda__1___boxed(lean_object*, lean_object*, lean_object*);
+LEAN_EXPORT lean_object* l_bricks__start__turn__from__ini__hist___boxed(lean_object*, lean_object*);
+LEAN_EXPORT lean_object* l_toy__strat(lean_object*, lean_object*);
+static lean_object* l_PickUpBricks__pubWin__vs__toy___closed__3;
+static lean_object* l_PickUpBricks__pubWin__vs__toy___closed__5;
+LEAN_EXPORT lean_object* l_pub__win__strat___boxed(lean_object*, lean_object*);
+uint8_t lean_nat_dec_eq(lean_object*, lean_object*);
+LEAN_EXPORT lean_object* l___private_Games_games_PickUpBricks_0__History__on__turn_match__1_splitter___rarg___boxed(lean_object*, lean_object*, lean_object*);
+LEAN_EXPORT lean_object* l_bricks__end__turn__from__ini__hist__act___boxed(lean_object*, lean_object*, lean_object*);
+lean_object* lean_nat_mod(lean_object*, lean_object*);
+LEAN_EXPORT lean_object* l_bricks__start__turn__from__ini__hist(lean_object*, lean_object*);
+static lean_object* l_PickUpBricks__pubWin__vs__toy___closed__1;
+LEAN_EXPORT lean_object* l___private_Games_games_PickUpBricks_0__History__on__turn_match__1_splitter(lean_object*);
+lean_object* lean_nat_sub(lean_object*, lean_object*);
+LEAN_EXPORT lean_object* l___private_Games_games_PickUpBricks_0__PickUpBricks_match__1_splitter___rarg(lean_object*, lean_object*, lean_object*, lean_object*);
+LEAN_EXPORT lean_object* l_pub__win__strat(lean_object*, lean_object*);
+LEAN_EXPORT lean_object* l_PickUpBricks(lean_object*);
+LEAN_EXPORT lean_object* l_PickUpBricks___elambda__1(lean_object*, lean_object*, lean_object*);
+LEAN_EXPORT lean_object* l_PickUpBricks__pubWin__vs__toy;
+LEAN_EXPORT lean_object* l_bricks__start__turn__from__ini__hist(lean_object* x_1, lean_object* x_2) {
+_start:
+{
+lean_object* x_3; lean_object* x_4; lean_object* x_5; 
+x_3 = lean_unsigned_to_nat(0u);
+x_4 = l_List_foldl___at_Composition_sizeUpTo___spec__2(x_3, x_2);
+x_5 = lean_nat_sub(x_1, x_4);
+lean_dec(x_4);
+return x_5;
+}
+}
+LEAN_EXPORT lean_object* l_bricks__start__turn__from__ini__hist___boxed(lean_object* x_1, lean_object* x_2) {
+_start:
+{
+lean_object* x_3; 
+x_3 = l_bricks__start__turn__from__ini__hist(x_1, x_2);
+lean_dec(x_2);
+lean_dec(x_1);
+return x_3;
+}
+}
+LEAN_EXPORT lean_object* l_bricks__end__turn__from__ini__hist__act(lean_object* x_1, lean_object* x_2, lean_object* x_3) {
+_start:
+{
+lean_object* x_4; lean_object* x_5; lean_object* x_6; lean_object* x_7; 
+x_4 = lean_unsigned_to_nat(0u);
+x_5 = l_List_foldl___at_Composition_sizeUpTo___spec__2(x_4, x_2);
+x_6 = lean_nat_sub(x_1, x_5);
+lean_dec(x_5);
+x_7 = lean_nat_sub(x_6, x_3);
+lean_dec(x_6);
+return x_7;
+}
+}
+LEAN_EXPORT lean_object* l_bricks__end__turn__from__ini__hist__act___boxed(lean_object* x_1, lean_object* x_2, lean_object* x_3) {
+_start:
+{
+lean_object* x_4; 
+x_4 = l_bricks__end__turn__from__ini__hist__act(x_1, x_2, x_3);
+lean_dec(x_3);
+lean_dec(x_2);
+lean_dec(x_1);
+return x_4;
+}
+}
+LEAN_EXPORT lean_object* l_PickUpBricks___elambda__1(lean_object* x_1, lean_object* x_2, lean_object* x_3) {
+_start:
+{
+lean_object* x_4; lean_object* x_5; lean_object* x_6; lean_object* x_7; 
+x_4 = lean_unsigned_to_nat(0u);
+x_5 = l_List_foldl___at_Composition_sizeUpTo___spec__2(x_4, x_2);
+x_6 = lean_nat_sub(x_1, x_5);
+lean_dec(x_5);
+x_7 = lean_nat_sub(x_6, x_3);
+lean_dec(x_6);
+return x_7;
+}
+}
+LEAN_EXPORT lean_object* l_PickUpBricks(lean_object* x_1) {
+_start:
+{
+lean_object* x_2; lean_object* x_3; 
+lean_inc(x_1);
+x_2 = lean_alloc_closure((void*)(l_PickUpBricks___elambda__1___boxed), 3, 1);
+lean_closure_set(x_2, 0, x_1);
+x_3 = lean_alloc_ctor(0, 2, 0);
+lean_ctor_set(x_3, 0, x_1);
+lean_ctor_set(x_3, 1, x_2);
+return x_3;
+}
+}
+LEAN_EXPORT lean_object* l_PickUpBricks___elambda__1___boxed(lean_object* x_1, lean_object* x_2, lean_object* x_3) {
+_start:
+{
+lean_object* x_4; 
+x_4 = l_PickUpBricks___elambda__1(x_1, x_2, x_3);
+lean_dec(x_3);
+lean_dec(x_2);
+lean_dec(x_1);
+return x_4;
+}
+}
+LEAN_EXPORT lean_object* l_pub__win__strat(lean_object* x_1, lean_object* x_2) {
+_start:
+{
+lean_object* x_3; lean_object* x_4; lean_object* x_5; lean_object* x_6; lean_object* x_7; uint8_t x_8; 
+x_3 = lean_unsigned_to_nat(0u);
+x_4 = l_List_foldl___at_Composition_sizeUpTo___spec__2(x_3, x_2);
+x_5 = lean_nat_sub(x_1, x_4);
+lean_dec(x_4);
+x_6 = lean_unsigned_to_nat(3u);
+x_7 = lean_nat_mod(x_5, x_6);
+x_8 = lean_nat_dec_eq(x_5, x_3);
+lean_dec(x_5);
+if (x_8 == 0)
+{
+lean_object* x_9; uint8_t x_10; 
+x_9 = lean_unsigned_to_nat(1u);
+x_10 = lean_nat_dec_eq(x_7, x_9);
+lean_dec(x_7);
+if (x_10 == 0)
+{
+lean_object* x_11; 
+x_11 = lean_unsigned_to_nat(2u);
+return x_11;
+}
+else
+{
+lean_object* x_12; 
+x_12 = lean_unsigned_to_nat(1u);
+return x_12;
+}
+}
+else
+{
+lean_object* x_13; 
+lean_dec(x_7);
+x_13 = lean_unsigned_to_nat(0u);
+return x_13;
+}
+}
+}
+LEAN_EXPORT lean_object* l_pub__win__strat___boxed(lean_object* x_1, lean_object* x_2) {
+_start:
+{
+lean_object* x_3; 
+x_3 = l_pub__win__strat(x_1, x_2);
+lean_dec(x_2);
+lean_dec(x_1);
+return x_3;
+}
+}
+LEAN_EXPORT lean_object* l___private_Games_games_PickUpBricks_0__PickUpBricks_match__1_splitter___rarg(lean_object* x_1, lean_object* x_2, lean_object* x_3, lean_object* x_4) {
+_start:
+{
+lean_object* x_5; uint8_t x_6; 
+x_5 = lean_unsigned_to_nat(0u);
+x_6 = lean_nat_dec_eq(x_1, x_5);
+if (x_6 == 0)
+{
+lean_object* x_7; uint8_t x_8; 
+lean_dec(x_2);
+x_7 = lean_unsigned_to_nat(1u);
+x_8 = lean_nat_dec_eq(x_1, x_7);
+if (x_8 == 0)
+{
+lean_object* x_9; 
+lean_dec(x_3);
+x_9 = lean_apply_4(x_4, x_1, lean_box(0), lean_box(0), lean_box(0));
+return x_9;
+}
+else
+{
+lean_object* x_10; 
+lean_dec(x_4);
+lean_dec(x_1);
+x_10 = lean_apply_1(x_3, lean_box(0));
+return x_10;
+}
+}
+else
+{
+lean_object* x_11; 
+lean_dec(x_4);
+lean_dec(x_3);
+lean_dec(x_1);
+x_11 = lean_apply_1(x_2, lean_box(0));
+return x_11;
+}
+}
+}
+LEAN_EXPORT lean_object* l___private_Games_games_PickUpBricks_0__PickUpBricks_match__1_splitter(lean_object* x_1) {
+_start:
+{
+lean_object* x_2; 
+x_2 = lean_alloc_closure((void*)(l___private_Games_games_PickUpBricks_0__PickUpBricks_match__1_splitter___rarg), 4, 0);
+return x_2;
+}
+}
+LEAN_EXPORT lean_object* l_toy__strat(lean_object* x_1, lean_object* x_2) {
+_start:
+{
+lean_object* x_3; lean_object* x_4; lean_object* x_5; uint8_t x_6; 
+x_3 = lean_unsigned_to_nat(0u);
+x_4 = l_List_foldl___at_Composition_sizeUpTo___spec__2(x_3, x_2);
+x_5 = lean_nat_sub(x_1, x_4);
+lean_dec(x_4);
+x_6 = lean_nat_dec_eq(x_5, x_3);
+lean_dec(x_5);
+if (x_6 == 0)
+{
+lean_object* x_7; 
+x_7 = lean_unsigned_to_nat(1u);
+return x_7;
+}
+else
+{
+lean_object* x_8; 
+x_8 = lean_unsigned_to_nat(0u);
+return x_8;
+}
+}
+}
+LEAN_EXPORT lean_object* l_toy__strat___boxed(lean_object* x_1, lean_object* x_2) {
+_start:
+{
+lean_object* x_3; 
+x_3 = l_toy__strat(x_1, x_2);
+lean_dec(x_2);
+lean_dec(x_1);
+return x_3;
+}
+}
+static lean_object* _init_l_PickUpBricks__pubWin__vs__toy___closed__1() {
+_start:
+{
+lean_object* x_1; lean_object* x_2; 
+x_1 = lean_unsigned_to_nat(32u);
+x_2 = lean_alloc_closure((void*)(l_PickUpBricks___elambda__1___boxed), 3, 1);
+lean_closure_set(x_2, 0, x_1);
+return x_2;
+}
+}
+static lean_object* _init_l_PickUpBricks__pubWin__vs__toy___closed__2() {
+_start:
+{
+lean_object* x_1; lean_object* x_2; lean_object* x_3; 
+x_1 = lean_unsigned_to_nat(32u);
+x_2 = l_PickUpBricks__pubWin__vs__toy___closed__1;
+x_3 = lean_alloc_ctor(0, 2, 0);
+lean_ctor_set(x_3, 0, x_1);
+lean_ctor_set(x_3, 1, x_2);
+return x_3;
+}
+}
+static lean_object* _init_l_PickUpBricks__pubWin__vs__toy___closed__3() {
+_start:
+{
+lean_object* x_1; 
+x_1 = lean_alloc_closure((void*)(l_pub__win__strat___boxed), 2, 0);
+return x_1;
+}
+}
+static lean_object* _init_l_PickUpBricks__pubWin__vs__toy___closed__4() {
+_start:
+{
+lean_object* x_1; 
+x_1 = lean_alloc_closure((void*)(l_toy__strat___boxed), 2, 0);
+return x_1;
+}
+}
+static lean_object* _init_l_PickUpBricks__pubWin__vs__toy___closed__5() {
+_start:
+{
+lean_object* x_1; lean_object* x_2; lean_object* x_3; lean_object* x_4; 
+x_1 = l_PickUpBricks__pubWin__vs__toy___closed__2;
+x_2 = l_PickUpBricks__pubWin__vs__toy___closed__3;
+x_3 = l_PickUpBricks__pubWin__vs__toy___closed__4;
+x_4 = lean_alloc_ctor(0, 3, 0);
+lean_ctor_set(x_4, 0, x_1);
+lean_ctor_set(x_4, 1, x_2);
+lean_ctor_set(x_4, 2, x_3);
+return x_4;
+}
+}
+static lean_object* _init_l_PickUpBricks__pubWin__vs__toy() {
+_start:
+{
+lean_object* x_1; 
+x_1 = l_PickUpBricks__pubWin__vs__toy___closed__5;
+return x_1;
+}
+}
+LEAN_EXPORT lean_object* l___private_Games_games_PickUpBricks_0__History__on__turn_match__1_splitter___rarg(lean_object* x_1, lean_object* x_2, lean_object* x_3) {
+_start:
+{
+lean_object* x_4; uint8_t x_5; 
+x_4 = lean_unsigned_to_nat(0u);
+x_5 = lean_nat_dec_eq(x_1, x_4);
+if (x_5 == 0)
+{
+lean_object* x_6; lean_object* x_7; lean_object* x_8; 
+x_6 = lean_unsigned_to_nat(1u);
+x_7 = lean_nat_sub(x_1, x_6);
+x_8 = lean_apply_1(x_3, x_7);
+return x_8;
+}
+else
+{
+lean_dec(x_3);
+lean_inc(x_2);
+return x_2;
+}
+}
+}
+LEAN_EXPORT lean_object* l___private_Games_games_PickUpBricks_0__History__on__turn_match__1_splitter(lean_object* x_1) {
+_start:
+{
+lean_object* x_2; 
+x_2 = lean_alloc_closure((void*)(l___private_Games_games_PickUpBricks_0__History__on__turn_match__1_splitter___rarg___boxed), 3, 0);
+return x_2;
+}
+}
+LEAN_EXPORT lean_object* l___private_Games_games_PickUpBricks_0__History__on__turn_match__1_splitter___rarg___boxed(lean_object* x_1, lean_object* x_2, lean_object* x_3) {
+_start:
+{
+lean_object* x_4; 
+x_4 = l___private_Games_games_PickUpBricks_0__History__on__turn_match__1_splitter___rarg(x_1, x_2, x_3);
+lean_dec(x_2);
+lean_dec(x_1);
+return x_4;
+}
+}
+lean_object* initialize_Init(uint8_t builtin, lean_object*);
+lean_object* initialize_Games_exLib_Nat(uint8_t builtin, lean_object*);
+lean_object* initialize_Games_gameLib_Basic(uint8_t builtin, lean_object*);
+lean_object* initialize_Mathlib_Tactic(uint8_t builtin, lean_object*);
+static bool _G_initialized = false;
+LEAN_EXPORT lean_object* initialize_Games_games_PickUpBricks(uint8_t builtin, lean_object* w) {
+lean_object * res;
+if (_G_initialized) return lean_io_result_mk_ok(lean_box(0));
+_G_initialized = true;
+res = initialize_Init(builtin, lean_io_mk_world());
+if (lean_io_result_is_error(res)) return res;
+lean_dec_ref(res);
+res = initialize_Games_exLib_Nat(builtin, lean_io_mk_world());
+if (lean_io_result_is_error(res)) return res;
+lean_dec_ref(res);
+res = initialize_Games_gameLib_Basic(builtin, lean_io_mk_world());
+if (lean_io_result_is_error(res)) return res;
+lean_dec_ref(res);
+res = initialize_Mathlib_Tactic(builtin, lean_io_mk_world());
+if (lean_io_result_is_error(res)) return res;
+lean_dec_ref(res);
+l_PickUpBricks__pubWin__vs__toy___closed__1 = _init_l_PickUpBricks__pubWin__vs__toy___closed__1();
+lean_mark_persistent(l_PickUpBricks__pubWin__vs__toy___closed__1);
+l_PickUpBricks__pubWin__vs__toy___closed__2 = _init_l_PickUpBricks__pubWin__vs__toy___closed__2();
+lean_mark_persistent(l_PickUpBricks__pubWin__vs__toy___closed__2);
+l_PickUpBricks__pubWin__vs__toy___closed__3 = _init_l_PickUpBricks__pubWin__vs__toy___closed__3();
+lean_mark_persistent(l_PickUpBricks__pubWin__vs__toy___closed__3);
+l_PickUpBricks__pubWin__vs__toy___closed__4 = _init_l_PickUpBricks__pubWin__vs__toy___closed__4();
+lean_mark_persistent(l_PickUpBricks__pubWin__vs__toy___closed__4);
+l_PickUpBricks__pubWin__vs__toy___closed__5 = _init_l_PickUpBricks__pubWin__vs__toy___closed__5();
+lean_mark_persistent(l_PickUpBricks__pubWin__vs__toy___closed__5);
+l_PickUpBricks__pubWin__vs__toy = _init_l_PickUpBricks__pubWin__vs__toy();
+lean_mark_persistent(l_PickUpBricks__pubWin__vs__toy);
+return lean_io_result_mk_ok(lean_box(0));
+}
+#ifdef __cplusplus
+}
+#endif
