Games/gameLib/Careless_Example.lean
@@ -1,0 +1,34 @@
+/-
+Copyright (c) 2024 Yves Jäckle. All rights reserved.
+Released under Apache 2.0 license as described in the file LICENSE.
+Author: Yves Jäckle.
+-/
+
+import Games.gameLib.Zermelo
+import Games.games.PickUpBricks
+
+def careful_strat (ini : ℕ) (hist : List ℕ) :=
+  if bricks_start_turn_from_ini_hist ini hist = 0
+  then 0
+  else if hist = []
+       then 1
+       else 2
+
+
+#eval History_on_turn 10 toy_strat careful_strat 10
+-- recall that toy strat always takes 1 brick
+#eval (History_on_turn 9 careful_strat toy_strat 9) ++ [toy_strat 10 []]
+-- the histories are different
+
+
+def careful_strat' (ini : ℕ) (hist : List ℕ) :=
+  if bricks_start_turn_from_ini_hist ini hist = 0
+  then 0
+  else if hist.length < 3
+       then 1
+       else 2
+
+
+#eval History_on_turn 10 toy_strat careful_strat' 10
+-- The histories coincide for the first few turn, but are differ later on
+#eval (History_on_turn 9 careful_strat' toy_strat 10) ++ [toy_strat 10 []]
