Games/games/TicTacToe.lean
@@ -1,0 +1,60 @@
+/-
+Copyright (c) 2024 Yves Jäckle. All rights reserved.
+Released under Apache 2.0 license as described in the file LICENSE.
+Author: Yves Jäckle.
+-/
+
+import Games.gameLib.Basic
+
+
+variable (D n : ℕ)
+
+inductive in_de_const (s : Fin n → Fin n) : Prop
+| cst : (∃ x : Fin n, ∀ i : Fin n, s i = x) → in_de_const s
+| inc : (∀ i : Fin n, s i = i) → in_de_const s
+| dec : (∀ i : Fin n, s i = n - 1 - i) → in_de_const s
+
+
+structure seq_is_line (s : Fin n → (Fin D → Fin n)) : Prop where
+  idc : ∀ d : Fin D, in_de_const n (fun j : Fin n => (s j) d)
+  non_pt : ¬ (∀ d : Fin D, (∃ x : Fin n, ∀ j : Fin n, s j d = x))
+
+
+def has_x_line (state : ((Fin D → Fin n) → Fin 3)) : Prop :=
+  ∃ l : Fin n → (Fin D → Fin n), (seq_is_line D n l) ∧ (∀ i : Fin n, state (l i) = 1)
+
+
+def has_o_line (state : ((Fin D → Fin n) → Fin 3)) : Prop :=
+  ∃ l : Fin n → (Fin D → Fin n), (seq_is_line D n l) ∧ (∀ i : Fin n, state (l i) = 2)
+
+
+def TTT_fst_trans (hist : List (Fin D → Fin n)) (act : (Fin D → Fin n)) : (Fin D → Fin n) → Fin 3 :=
+  fun p => if h1 : p = act
+           then 1
+           else if h2 : p ∈ hist
+                then if h2a : Turn_fst (hist.indexOf p)
+                     then 1
+                     else 2
+                else 0
+
+def TTT_snd_trans (hist : List (Fin D → Fin n)) (act : (Fin D → Fin n)) : (Fin D → Fin n) → Fin 3 :=
+  fun p => if h1 : p = act
+           then 2
+           else if h2 : p ∈ hist
+                then if h2a : Turn_fst (hist.indexOf p)
+                     then 1
+                     else 2
+                else 0
+
+
+def TTT_legal (hist : List (Fin D → Fin n)) (act : (Fin D → Fin n)) : Prop := act ∉ hist
+
+
+def TTT : Game_World ((Fin D → Fin n) → Fin 3) (Fin D → Fin n) where
+  init_game_state := fun _ => 0
+  fst_win_states := fun s => has_x_line D n s
+  fst_transition := TTT_fst_trans D n
+  fst_legal := TTT_legal D n
+  snd_win_states := fun s => has_o_line D n s
+  snd_transition := TTT_snd_trans D n
+  snd_legal := TTT_legal D n
